set up ghost state for allocator

theories/iris/allocator/blocks.v
@@ -7,14 +7,17 @@ Inductive state_flag :=
 
 Inductive block : Type :=
 | UsedBlk
+    (base_addr: N)
     (blk_used_size: N)
     (blk_leftover_size: N)
     (*(blk_padding: iProp Σ)*)
 | FreeBlk
+    (base_addr: N)
     (blk_size: N).
 
 Inductive final_block : Type :=
 | FinalBlk
+    (base_addr: N)
     (blk_size: N).
 
 Definition blocks : Type :=
@@ -22,17 +25,33 @@ Definition blocks : Type :=
 
 Definition block_flag blk :=
   match blk with
-  | UsedBlk _ _ => Used
-  | FreeBlk _ => Free
+  | UsedBlk _ _ _ => Used
+  | FreeBlk _ _ => Free
   end.
 
 Definition final_block_flag blk :=
   match blk with
-  | FinalBlk _ => Final
+  | FinalBlk _ _ => Final
   end.
 
 Definition block_size blk : N :=
   match blk with
-  | UsedBlk sz_u sz_l => sz_u + sz_l
-  | FreeBlk sz => sz
+  | UsedBlk _ sz_u sz_l => sz_u + sz_l
+  | FreeBlk _ sz => sz
+  end.
+
+Definition block_addr blk : N :=
+  match blk with
+  | UsedBlk base_addr _ _
+  | FreeBlk base_addr _ => base_addr
+  end.
+
+Definition final_block_sz (blk: final_block) : N :=
+  match blk with
+  | FinalBlk _ sz => sz
+  end.
+
+Definition final_block_addr (blk: final_block) : N :=
+  match blk with
+  | FinalBlk addr _ => addr
   end.
