theories/iris/allocator/memrsc.v
@@ -6,6 +6,7 @@ From iris.base_logic.lib Require Export fancy_updates.
 From iris.bi Require Export weakestpre.
 From Wasm.iris.logrel Require Export iris_fundamental.
 From Wasm.iris.rules Require Export proofmode.
+Require Import RWasm.iris.allocator.misc_relocate.
 
 Section memrsc.
 Context `{!wasmG Σ}. 
@@ -13,4 +14,49 @@ Context `{!wasmG Σ}.
 Definition own_vec (memidx: N) (base_addr: N) (sz: N) : iProp Σ :=
   ∃ bs: bytes, ⌜N.of_nat (length bs) = sz⌝ ∗ memidx ↦[wms][base_addr] bs.
 
+Lemma own_vec_split memidx ℓ sz1 sz2 :
+  own_vec memidx ℓ (sz1 + sz2) ⊣⊢ own_vec memidx ℓ sz1 ∗ own_vec memidx (ℓ + sz1) sz2.
+Proof.
+  unfold own_vec.
+  iSplit.
+  - iIntros "(%bs & %Hlen & Hbs)".
+    pose proof (take_drop (N.to_nat sz1) bs) as Hsplit.
+    rewrite <- Hsplit.
+    rewrite wms_app; [|eauto; lia].
+    iDestruct "Hbs" as "(Hbs1 & Hbs2)".
+    iSplitL "Hbs1".
+    + iExists _; iFrame.
+      iPureIntro.
+      rewrite length_take_le; lia.
+    + rewrite length_take_le; [|lia].
+      rewrite N2Nat.id.
+      iExists _; iFrame.
+      iPureIntro.
+      rewrite length_drop.
+      lia.
+  - iIntros "((%bs1 & (%Hlen1 & Hbs1)) & (%bs2 & (%Hlen2 & Hbs2)))".
+    iExists (bs1 ++ bs2).
+    erewrite (wms_app _ _ _ (sz1:=sz1)); [| lia].
+    iFrame.
+    iPureIntro.
+    rewrite length_app.
+    lia.
+Qed.
+
+Class allocG Σ := {
+  (* maps locs returned by malloc to their size *)
+  allocG_shapeG :: ghost_mapG Σ N N;
+  allocG_shape : gname
+}.
+
 End memrsc.
+
+(* Authoritative shape map *)
+Notation "↪[toks] m" := (ghost_map_auth allocG_shape 1%Qp m)%I
+  (at level 20, format "↪[toks] m") : bi_scope.
+
+(* Atomic fragments of the shape map *)
+Notation "n ↦[tok]{ dq } sz" := (n ↪[allocG_shape]{dq} sz)%I
+  (at level 20, format "n ↦[tok]{ dq } sz") : bi_scope.
+Notation "n ↦[tok] sz" := (n ↪[allocG_shape]{(DfracOwn 1)} sz)%I
+  (at level 20, format "n ↦[tok] sz") : bi_scope.
